acl2s-raw/testing3.lisp
@@ -1,0 +1,122 @@
+(defttag t)
+
+(include-book "top" :uncertified-okp t)
+
+(defdata2 loi (listof integer))
+
+
+(defunc2 find-max (ls)
+  :input-contract (loip ls)
+  :output-contract (integerp (find-max ls))
+  (cond
+   ((endp ls) -100)
+   ((loip ls)
+    (let ((res (find-max (cdr ls)))
+	  (a (car ls)))
+      (if (> a res)
+	  a res)))))
+
+
+(suggest-lemma -100 :with find-max boolean)
+
+
+(defdata2
+  (inc-expr (list 'inc expr))
+  (let-expr (list 'let var expr expr))
+  (expr (oneof var nat inc-expr let-expr)))
+
+(defdata2 asst (alistof var nat))
+
+(defthm inc-cadr
+  (implies (inc-exprp e)
+	   (exprp (cadr e))))
+
+(defthm inc-cons (implies (inc-exprp e) (consp (cdr e))))
+
+(defthm let-cadr
+  (implies (let-exprp e)
+	   (exprp (cadr e))))
+
+(defthm let-caddr
+  (implies (let-exprp e)
+	   (exprp (caddr e))))
+
+(defthm let-cons
+  (implies (let-exprp e) (consp (cdr e))))
+
+(defthm let-cons2
+  (implies (let-exprp e) (consp (cddr e))))
+
+(defdata-disjoint inc-expr let-expr)
+
+
+
+(defunc2 assv (x ls)
+  :input-contract (and (varp x) (asstp ls))
+  :output-contract (or (equal (assv x ls) nil)
+		       (consp (assv x ls)))
+  (cond
+   ((endp ls) nil)
+   ((equal x (car (car ls))) (car ls))
+   (t (assv x (cdr ls)))))
+
+
+(suggest-lemma (assv x ls) :with assv)
+
+
+(defunc2 closedp (exp vars)
+  :input-contract (and (exprp exp) (asstp vars))
+  :output-contract (booleanp (closedp exp vars))
+  (cond
+   ((natp exp) t)
+   ((varp exp) (if (assv exp vars) t nil))
+   ((inc-exprp exp) (closedp (car (cdr exp)) vars))
+   ((let-exprp exp)
+    (let ((x (car (cdr exp)))
+	  (a (car (cdr (cdr exp))))
+	  (body (car (cdr (cdr (cdr exp))))))
+      (let ((new-vars (cons (cons x 0) vars)))
+	(and (closedp a vars)
+	     (closedp body new-vars)))))))
+
+(defthm inc-all
+  (implies (inc-exprp x)
+	   (and (consp x)
+		(consp (cdr x))
+		(exprp (cadr x)))))
+
+(defthm nat-exp
+  (implies (natp e) (exprp e)))
+
+(defthm destruct-expr
+  (equal (exprp e)
+	 (or (natp e)
+	     (varp e)
+	     (inc-exprp e)
+	     (let-exprp e))))
+
+(in-theory (disable exprp))
+
+(defunc2 eval-expr (exp rho)
+  :input-contract (and (exprp exp) (asstp rho))
+  :output-contract (natp (eval-expr exp rho))
+  (cond
+   ((natp exp) exp)
+   ((varp exp)
+    (let ((v (assv exp rho)))
+      (if v (cdr v) 0)))
+   ((inc-exprp exp)
+    (+ 1 (eval-expr 0 rho)))
+   #|((let-exprp exp)
+   (let* ((x (car (cdr exp)))
+   (a (car (cdr (cdr exp))))
+   (b (car (cdr (cdr (cdr exp))))))
+   (let ((a-v (eval-expr a rho)))
+   (let ((new-rho (cons (cons x a-v) rho)))
+      (eval-expr b new-rho)))))|#
+   (t 0)))
+
+
+(suggest-lemma 4
+	       :required-expressions eval-expr
+	       :with number)
