acl2s-raw/compile-defdata-raw.lsp
@@ -1,0 +1,234 @@
+(in-package "ACL2S")
+
+#|
+(load "helpers-raw.lsp")
+(load "mk-raw.lsp")
+(load "numbers-raw.lsp")
+(load "primitives-raw.lsp")
+|#
+(defun all-types ()
+  '((nat natpo natpo-fn)
+    (pos pospo pospo-fn)
+    (neg negpo negpo-fn)
+    (integer integerpo integerpo-fn)
+    (rational rationalpo rationalpo-fn)
+    (number numberpo numberpo-fn)
+    (symbol symbolpo symbolpo-fn)
+    (var varpo varpo-fn)
+    (string stringpo stringpo-fn)
+    (character charpo charpo-fn)
+    (cons conspo conspo-fn)
+    (list listpo listpo-fn)
+    (true-list true-listpo true-listpo-fn)))
+
+(defun defdata-make-val (exp)
+  (cond
+   ((booleanp exp) exp)
+   ((symbolp exp) (build-sym exp))
+   ((characterp exp) (build-char exp))
+   ((stringp exp) (build-string exp))
+   ((rationalp exp) (build-num exp))
+   ((consp exp)
+    (list 'INTERNAL-CONS (defdata-make-val (car exp))
+	  (defdata-make-val (cdr exp))))))
+
+(defun desugar-list (es)
+  (cond
+   ((endp es) nil)
+   (t `(cons ,(car es)
+	     ,(desugar-list (cdr es))))))
+
+(defun desugar-list* (es)
+  (cond
+   ((endp es) nil)
+   ((endp (cdr es)) (car es))
+   (t `(cons ,(car es)
+	     ,(desugar-list* (cdr es))))))
+
+
+(defun clean-range (n)
+  (cond
+   ((numberp n) (build-num n))
+   (t (let ((_ (ld `((assign result ,n)))))
+	(build-num (@ result))))))
+
+(defun finish-range (input lt lte gt gte)
+  (let ((gt-exp (mapcar #'(lambda (e)`(do-less-than-o ',e ,input)) gt))
+	(gte-exp (mapcar #'(lambda (e) `(do-less-than-equal-o ',e ,input)) gte))
+	(lt-exp (mapcar #'(lambda (e) `(do-less-than-o ,input ',e)) lt))
+	(lte-exp (mapcar #'(lambda (e) `(do-less-than-equal-o ,input ',e)) lte)))
+    `(conj ,(append lt-exp lte-exp gt-exp gte-exp))))
+
+
+(defun compile-range-3 (v1 v2 cmp input)
+  (cond
+   ((and (equal v1 '_) (equal cmp '<))
+    (finish-range input (list (clean-range v2)) nil nil nil))
+   ((and (equal v1 '_) (equal cmp '<=))
+    (finish-range input nil (list (clean-range v2)) nil nil))
+   ((and (equal v2 '_) (equal cmp '<))
+    (finish-range input nil nil (list (clean-range v1)) nil))
+   ((and (equal v2 '_) (equal cmp '<=))
+    (finish-range input nil nil nil (list (clean-range v1))))))
+
+(defun compile-range-5 (v1 v2 cmp1 cmp2 input)
+  (cond
+   ((and (equal cmp1 '<) (equal cmp2 '<))
+    (finish-range input (list (clean-range v2)) nil
+		  (list (clean-range v1)) nil))
+   ((and (equal cmp1 '<) (equal cmp2 '<=))
+    (finish-range input nil (list (clean-range v2))
+		  (list (clean-range v1)) nil))
+   ((and (equal cmp1 '<=) (equal cmp2 '<))
+    (finish-range input (list (clean-range v2)) nil
+		  nil (list (clean-range v1))))
+   ((and (equal cmp1 '<=) (equal cmp2 '<=))
+    (finish-range input nil (list (clean-range v2))
+		  nil (list (clean-range v1))))))
+
+(defun compile-range (e input)
+  (cond
+   ;; if there is only one comparator
+   ((equal (len e) 3)
+    (let ((v1 (car e)) (cmp (cadr e)) (v2 (caddr e)))
+      (compile-range-3 v1 v2 cmp input)))
+   ((equal (len e) 5)
+    (let ((v1 (car e)) (v2 (cadddr (cdr e)))
+	  (cmp1 (cadr e)) (cmp2 (cadddr e)))
+      (if (not (equal (caddr e) '_))
+	  (error "Range expected the middle term to be '_")
+	(compile-range-5 v1 v2 cmp1 cmp2 input))))))
+
+(defun compile-defdata (expr input self)
+  (cond
+   ;; constants
+   ((booleanp expr) `(== ,expr ,input))
+   ((numberp expr) `(== ',(build-num expr) ,input))
+   ((characterp expr) `(== ',(build-char expr) ,input))
+   ((stringp expr) `(== ',(build-string expr) ,input))
+   ;; other type symbols (the type being made has been added to this list)
+   ((symbolp expr)
+    (let ((p (assoc expr (all-types))))
+      (if p `(,(cadr p) ,input)
+	(error "Unknown symbol ~s" expr))))
+   ((consp expr)
+    (cond
+     ;; constants under quote
+     ((equal (car expr) 'quote)
+      `(== ,input ',(defdata-make-val (cadr expr))))
+     ;; oneof -> disjunction
+     ((equal (car expr) 'oneof)
+      `(disj ,(mapcar #'(lambda (e)
+			  (compile-defdata e input self))
+		      (cdr expr))))
+     ((equal (car expr) 'cons)
+      (let ((e1 (next-var))
+	    (e2 (next-var)))
+	`(fresh (,e1 ,e2)
+		(conso ,e1 ,e2 ,input)
+		,(compile-defdata (cadr expr) e1 self)
+		,(compile-defdata (caddr expr) e2 self))))
+     ;; listof, list, and list*, and alistof can all just be desugared
+     ((equal (car expr) 'listof)
+      (let ((elem-type (cadr expr)))
+	`(disj2 (== ,input nil)
+		,(compile-defdata `(cons ,elem-type ,self) input self))))
+     ((equal (car expr) 'alistof)
+      (let ((key-type (cadr expr))
+	    (val-type (cadr expr)))
+	(compile-defdata `(listof (cons ,key-type ,val-type)) input self)))
+     ((equal (car expr) 'list)
+      (compile-defdata (desugar-list (cdr expr)) input self))
+     ((equal (car expr) 'list*)
+      (compile-defdata (desugar-list* (cdr expr)) input self))
+     ((equal (car expr) 'range)
+      (let ((type (cadr expr))
+	    (range (caddr expr)))
+	(let* ((v (assoc type (all-types)))
+	       (vp (if v (cadr v) (error "Unknown range type ~s" type))))
+	  `(conj2 (,vp ,input)
+		  ,(compile-range range input)))))
+     ((equal (car expr) 'enum)
+      (let* ((_ (ld `((assign result ,(cadr expr)))))
+	     (ls (defdata-make-val (@ result))))
+	`(membero-fn ,input ',ls t)))
+     ;; Otherwise, it is some expression to be evaluated
+     (t (let ((_ (ld `((assign result ,expr)))))
+	  (compile-defdata `',(@ result) input self)))))
+   (t (error "Invalid datatype ~s" expr))))
+
+(defun defdata2-- (name expr)
+  (let* ((pred-name (get-pred-name name))
+	 (rel-name (get-rel-name pred-name)))
+    (let* ((input (next-var))
+	   (expr (compile-defdata expr input name)))
+      `(defrel ,rel-name (,input) ,expr))))
+
+(defun update-types (es)
+  (let ((ts (all-types))
+	(new (mapcar #'(lambda (x)
+			 (let ((p (get-pred-name x)))
+			   (list x (get-rel-name p) (get-rel-fn-name p))))
+		     es)))
+    (defun all-types ()
+      (append ts new))))
+
+
+(defun make-fn-version-clause (name)
+  `((,name e) (== o nil)))
+
+(defun make-fn-version (form)
+  (let* ((form-rel (get-rel-name form))
+	 (form-rel-fn (get-rel-fn-name form)))
+    `(defrel ,form-rel-fn (e o)
+       (conde
+	((,form-rel e) (== o t))
+	. ,(mapcar #'make-fn-version-clause
+		   (mapcar #'cadr (all-types)))))))
+
+
+#|
+(defun defdata2- (exprs)
+  (cond
+   ((endp exprs) (error "Defdata2 expected to receive arguments, received nothing"))
+   ;; single defs
+   ((symbolp (car exprs))
+    (progn
+      (update-types (list (car exprs)))
+      (defdata2-- (car exprs) (cadr exprs))))
+   ;; mutually recursive defs
+   (t (progn
+	(update-types (mapcar #'car exprs))
+	`(progn . ,(mapcar #'(lambda (a) (defdata2-- (car a) (cadr a)))
+			   exprs))))))
+|#
+#|
+(defdata2 '(foo (listof nat)))
+
+(defdata2 '(bar (oneof 0 1/2 (listof character))))
+
+
+(defdata2 '(expr
+	    (oneof (list 'load nat var)
+		    (list 'mult nat nat)
+		    (list 'add nat nat)
+		    (list 'pop var))))
+
+(defdata2
+  '((foo (oneof t nil))
+    (bar (oneof foo nat))))
+
+(defdata2 '(quo (oneof cons (append '(1 2) '(2 3)))))
+
+(defdata2 '(foo (range integer (3 < _ <= 7))))
+
+(defdata2 '(foo (range integer (3 <= _ < 5))))
+
+(defdata2 '(bar (range rational (_ <= 4/5))))
+
+(defdata2 '(bar (range nat (44 < _))))
+
+(defdata2 '(enum1 (enum '(1 2 3))))
+
+(defdata2 '(enum2 (enum (append nil nil nil nil nil))))
+|#
