acl2s-raw/compile-raw.lsp
@@ -1,14 +1,12 @@
-;(load "helpers-raw.lsp")
-
-;; Just a function for a common idiom
-(defun has-form (s e)
-  (and (consp e) (equal (car e) s)))
+(in-package "ACL2S")
 
 ;; Go: a guard to decide if recursion is necessary.
 (defun miniKanrenize-go (e)
   (cond
    ((symbolp e) `(nil ,e))
    ((numberp e) `(nil ',(build-num e)))
+   ((stringp e) `(nil ',(build-string e)))
+   ((characterp e) `(nil ',(build-char e)))
    (t (let ((v (next-var)))
 	(list t v (miniKanrenize e v))))))
 
@@ -33,6 +31,28 @@
 				    vars dest (cdr es) work
 				    has-dest?))))))
 
+(defun complete-recursion-inner-nary (form id dest es)
+  (cond
+   ((endp es) `(== ,id ,dest))
+   ((endp (cdr es))
+    (let ((curr (car es)))
+      (if (car curr)
+	  `(conj2 (== ,(cadr curr) ,dest) ,(caddr curr))
+	`(== ,(cadr curr) ,dest))))
+   ((endp (cddr es))
+    (let ((e1 (car es)) (e2 (cadr es)))
+      `(conj
+	(,@(append (cddr e1) (cddr e2))
+	 (,form ,(cadr e1) ,(cadr e2) ,dest)))))
+   (t (let* ((e1 (car es))
+	     (name-for-e1 (cadr e1))
+	     (work-for-e1 (cddr e1))
+	     (int (next-var)))
+	`(fresh (,int)
+		,(complete-recursion-inner-nary form id int (cdr es))
+		,@work-for-e1
+		(,form ,name-for-e1 ,int ,dest))))))
+
 (defun complete-recursion (form dest es)
   (complete-recursion-inner form nil dest es nil t))
 (defun complete-recursion-bool (form es)
@@ -43,27 +63,25 @@
 ;; cond and if call the recursive function miniKanrenize-bool, which
 ;; creates dest-less expressions not expected to generate output
 
-(defparameter built-ins
-  '((cons 2 conso) (car 1 caro) (cdr 1 cdro)
-    (append 2 appendo) (reverse 1 reverso) (len 1 leno)
-    (+ 2 do-pluso) (- 2 do-minuso) (* 2 do-timeso) (sqr 1 do-sqro)
-    (< 2 do-less-than-o-fn) (<= 2 do-less-than-equal-o-fn)
-    (> 2 do-greater-than-o-fn) (>= 2 do-greater-than-equal-o-fn)
-    (and nil ando) (or nil oro) (not 1 noto)
-    (booleanp 1 booleanpo-fn) (symbolp 1 symbolpo-fn)
-    (varp 1 varpo-fn) (consp 1 conspo-fn) (symbolp 1 symbolpo-fn)
-    (endp 1 endpo-fn) (equal 2 ==-fn)
-    ;; numbers (has changed)
-    (zerop 1 zeropo-fn) (numberp 1 numberpo-fn)
-    (natp 1 natpo-fn) (integerp 1 integerpo-fn) (posp 1 pospo-fn)
-    (negp 1 negpo-fn) (rationalp 1 rationalpo-fn)
-    (numerator 1 numeratoro) (denominator 1 denominatoro)
-    ;; strings and chars
-    (stringp 1 stringpo-fn) (characterp 1 charpo-fn)
-    (string-append 2 concato) (length 1 str-leno)
-    (subseq 3 subseqo)))
+(defun compiler-knows-function? (form)
+  (cond
+   ((equal form 'cons) '(2 conso))
+   ((equal form 'car) '(1 caro))
+   ((equal form 'cdr) '(1 cdro))
+   (t (function-is-known? form))))
 
 (defun do-rec (form es dest)
+  (let ((es (mapcar #'miniKanrenize-go es))
+	(v (compiler-knows-function? form)))
+    (let* ((arity (car v))
+	   (identity (cadr v))
+	   (rel-name (if arity (cdr v) (cddr v))))
+      (cond
+       ((not arity) (complete-recursion-inner-nary (car rel-name) identity dest es))
+       ((equal arity (length es)) (complete-recursion rel-name dest es))
+       (t (error "Wrong number of args given to ~a" form))))))
+
+#|(defun do-rec (form es dest)
   (let ((es (mapcar #'miniKanrenize-go es))
 	(v (assoc form built-ins)))
     (if v
@@ -72,14 +90,20 @@
 	  (error "Wrong number of args given to ~a" form))
       (let ((name (get-rel-name form)))
 	(complete-recursion `(,name) dest es)))))
-
+|#
 (defun miniKanrenize (expr dest)
   (cond
    ;; base cases
    ((booleanp expr) `(== ,expr ,dest))
    ((numberp expr) `(== ',(build-num expr) ,dest))
+   ((stringp expr) `(== ',(build-string expr) ,dest))
+   ((characterp expr) `(== ',(build-char expr) ,dest))
    ((symbolp expr) `(== ,expr ,dest))
-   ((has-form 'quote expr) `(== ',(build-sym expr) ,dest))
+   ((has-form 'quote expr) `(== ',(clean-val expr) ,dest))
+   ;; Since interp handles these separately, so does compile
+   ((has-form 'cons expr) (do-rec 'cons (cdr expr) dest))
+   ((has-form 'car expr) (do-rec 'car (cdr expr) dest))
+   ((has-form 'cdr expr) (do-rec 'cdr (cdr expr) dest))
    ;; Special cases: let, control flow
    ((has-form 'let expr) (miniKanrenize-let expr dest))
    ((has-form 'let* expr) (miniKanrenize-let* expr dest))
@@ -99,7 +123,7 @@
 ;; conditionals
 (defun miniKanrenize-cond (lines negations dest)
   (cond
-   ((endp lines) '(((fail))))
+   ((endp lines) `(((== ,dest nil))))
    (t (let* ((line1 (car lines))
 	     (test (miniKanrenize-bool (car line1)))
 	     (test-neg (miniKanrenize-bool `(not ,(car line1)))))
@@ -117,7 +141,6 @@
 					 (list t alt))
 				   nil
 				   dest))))
-
 ;; let statements
 
 (defun miniKanrenize-let (expr dest)
@@ -145,27 +168,20 @@
 		,(miniKanrenize e x)
 		,(miniKanrenize-let*- (cdr lines) body))))))
 
+
 ;; booleans
-(defparameter built-ins-bool
-  '((equal 2 ==)
-    (varp 1 varpo) (booleanp 1 booleanpo) (symbolp 1 symbolpo) (endp 1 endpo)
-    (consp 1 conspo) (stringp 1 stringpo) (characterp 1 charpo)
-    (< 2 do-less-than-o) (<= 2 do-less-than-equal-o)
-    (> 2 do-greater-than-o) (>= 2 do-greater-than-equal-o)
-    ;; numbers (has changed)
-    (zerop 1 zeropo) (numberp 1 numberpo)
-    (natp 1 natpo) (integerp 1 integerpo) (posp 1 pospo)
-    (negp 1 negpo) (rationalp 1 rationalpo)))
 
 (defun do-rec-bool (form es)
   (let ((es (mapcar #'miniKanrenize-go es))
-	(v (assoc form built-ins-bool)))
-    (if v
-	(if (or (not (cadr v)) (equal (length es) (cadr v)))
-	    (complete-recursion-bool (cddr v) es)
-	  (error "Wrong number of args given to ~a" form))
-      (let ((name (get-rel-name form)))
-	(complete-recursion-bool `(,name) es)))))
+	(v (function-is-known-bool? form)))
+    (let* ((arity (car v))
+	   (identity (cadr v))
+	   (rel-name (if arity (cdr v) (cddr v))))
+      (cond
+       ((not arity)
+	(complete-recursion-inner-nary (car rel-name) identity (next-var) es))
+       ((equal arity (length es)) (complete-recursion-bool rel-name es))
+       (t (error "Wrong number of args given to ~a" form))))))
 
 (defun miniKanrenize-bool (expr)
   (cond
@@ -174,6 +190,7 @@
    ((equal expr 'nil) '(fail))
    ((numberp expr) '(succeed))
    ((symbolp expr) '(succeed))
+   ((has-form 'quote expr) '(succeed))
    ;; standard ops with boolean versions
    ((and (consp expr)
 	 (assoc (car expr) built-ins-bool))
