acl2s-raw/defunc2-raw.lsp
@@ -1,11 +1,14 @@
 (in-package "ACL2S")
 
-(load "compile-raw.lsp")
-(load "to-acl2-raw.lsp")
+;(load "compile-raw.lsp")
+;(load "to-acl2-raw.lsp")
 #|
 (load "helpers-raw.lsp")
 (load "interp-raw.lsp")
+(load "compile-defdata-raw.lsp")
 |#
+
+;; defun core functions
 (defun gen-mk (name vars definition)
   (let ((new-output (next-var))
 	(new-name (get-rel-name name)))
@@ -13,20 +16,57 @@
       (eval `(defrel ,new-name ,(append vars (list new-output))
 	       ,a)))))
 
-(defun gen-rel-inner (name vars body state)
+(defun defunc2- (name vars body state)
   (progn
     (add-to-interpreter name (get-rel-name name) (len vars))
     (gen-mk name vars body)
     (mv nil nil state)))
 
+(defun add-all-to-built-ins (forms rel rel-fn)
+  (cond
+   ((endp forms) (defparameter built-ins-bool (append rel built-ins-bool)))
+   (t (let* ((f (car forms))
+	     (pf (get-pred-name f))
+	     (pf-rel (get-rel-name pf))
+	     (pf-fn (get-rel-fn-name pf)))
+	(add-to-interpreter pf pf-fn 1)
+	(add-all-to-built-ins (cdr forms)
+			      (cons `(,f 1 ,pf-rel) rel)
+			      (cons `(,f 1 ,pf-fn) rel-fn))))))
+
+;; defdata core functions
+(defun defdata2- (exprs)
+  (cond
+   ((endp exprs) (error "Defdata2 expected to receive arguments, received nothing"))
+   ;; single defs
+   ((symbolp (car exprs))
+    (let* ((name (car exprs))
+	   (pred-name (get-pred-name name))
+	   (rel-name (get-rel-name pred-name))
+	   (rel-fn-name (get-rel-fn-name pred-name)))
+      (progn
+	;; new type exists
+	(update-types (list name))
+	;; interpreter knows about fn-version
+	(add-to-interpreter pred-name rel-fn-name 1)
+	(defparameter built-ins-bool (cons `(,pred-name 1 ,rel-name) built-ins-bool))
+	(eval (defdata2-- (car exprs) (cadr exprs)))
+	(eval (make-fn-version pred-name)))))
+   ;; mutually recursive defs
+   (t (progn
+	(update-types (mapcar #'car exprs))
+	(add-all-to-built-ins (mapcar #'car exprs) nil nil)
+	(eval `(progn . ,(mapcar #'(lambda (a) (defdata2-- (car a) (cadr a)))
+				 exprs)))))))
+
 ;;;;; Creating new clauses for relational ACL2s interpreter
 
+;; has arity helps make better forms
 (defun has-arity-clause (name n)
   `((== form ',name) (== n ,n)))
 
 (defun add-to-interpreter (name rel-name num-args)
-  (let ((new-clause
-	 (new-clause num-args nil `(list ',name) nil `(,rel-name)))
+  (let ((new-clause (new-clause num-args nil `(list ',name) nil `(,rel-name)))
 	(new-arity-clause (has-arity-clause name num-args))
 	(current-interp (expr-for-value-of))
 	(current-lines (all-lines))
@@ -38,7 +78,14 @@
 	(append current-lines (list name)))
       (defun expr-for-has-arity ()
 	(append current-arities (list new-arity-clause)))
+      (defparameter built-ins (cons `(,name ,num-args ,rel-name) built-ins))
       (eval `(defrel value-of (expr ρ o)
 	       ,(expr-for-value-of)))
       (eval `(defrel has-arity (form n)
 	       ,(expr-for-has-arity))))))
+
+;; for some reason I keep needing to redefine this
+(defun all-lines ()
+  (append 
+   '(var boolean symbol number string char cons car cdr let if cond)
+   (mapcar #'car built-ins)))
