acl2s-raw/helpers-raw.lsp
@@ -1,5 +1,9 @@
 (in-package "ACL2S")
 
+;; Just a function for a common idiom
+(defun has-form (s e)
+  (and (consp e) (equal (car e) s)))
+
 ; Creating new variable names
 (defun next-index () 0)
 (defun next-var ()
@@ -28,5 +32,148 @@
 
 ;; The name of a miniKanrenized function
 (defun get-rel-name (name)
-  (intern
-   (concatenate 'string (string name) "-REL")))
+  (intern-in-package-of-symbol
+   (concatenate 'string (string name) "-REL")
+   'acl2s::allp))
+
+(defun get-rel-fn-name (name)
+  (intern-in-package-of-symbol
+   (concatenate 'string (string name) "-REL-FN")
+   'acl2s::allp))
+
+(defun get-pred-name (name)
+  (intern-in-package-of-symbol (concatenate 'string (string name) "P")
+			       'acl2s::allp))
+;; functions for converting ACL2S values to MK values
+
+(defun fix-atom (e)
+  (cond
+   ((symbolp e) e)
+   ((characterp e) (build-char e))
+   ((stringp e) (build-string e))
+   ((rationalp e) (build-num e))
+   ;; complex numbers become nil
+   (t nil)))
+
+
+;; add tags to quoted values, creating valid expressions
+(defun fix-values (e)
+  (cond
+   ((consp e)
+    `(cons ,(fix-values (car e))
+	   ,(fix-values (cdr e))))
+   ((booleanp e) e)
+   ((symbolp e) (build-sym e))
+   (t (fix-atom e))))
+
+;; take input expressions, find quoted terms (and numbers), and fix.
+;; uses values->expressions under quote, and otherwise only changes numbers
+(defun clean-expr (e)
+  (cond
+   ((not (consp e)) (fix-atom e))
+   ((equal (car e) 'quote) (fix-values (cadr e)))
+   (t (cons (clean-expr (car e))
+	    (clean-expr (cdr e))))))
+
+;;;;;;;;;;;;;;;;;;;;;;;;;;;;;;;;;;;;;;;;;;;;;;;;;
+;; forms to create valid values from test cases (for environment)
+
+(defun elim-quote (exp)
+  (cond
+   ((symbolp exp) exp)
+   ((not (consp exp)) exp)
+   ((equal (car exp) 'quote) (elim-quote (cadr exp)))
+   (t (cons (elim-quote (car exp))
+	    (elim-quote (cdr exp))))))
+
+(defun coerce-val (pr)
+  (list (car pr) (elim-quote (cadr pr))))
+
+(defun coerce-tests (tests)
+  (mapcar #'coerce-val tests))
+
+(defun clean-val (exp)
+  (cond
+   ((booleanp exp) exp)
+   ((symbolp exp) (build-sym exp))
+   ((not (consp exp)) (fix-atom exp))
+   ((equal (car exp) 'quote) (clean-val (cadr exp)))
+   ((consp exp)
+    (list 'INTERNAL-CONS (clean-val (car exp))
+	  (clean-val (cdr exp))))))
+
+(defun clean-pr (pr)
+  (list (car pr) (clean-val (cadr pr))))
+
+(defun clean-tests (alist) (mapcar #'clean-pr alist))
+
+;;; Takes synthesized expressions, and removes evidence
+;; of internal values
+(defun read-back (v)
+  (cond
+   ((symbolp v) v)
+   ((consp v)
+    (let ((tag (car v)))
+      (cond
+       ((equal tag 'INTERNAL-SYMBOL) (cadr v))
+       ((equal tag 'INTERNAL-VARSYMBOL) (cadr v))
+       ((equal tag 'INTERNAL-CHAR) (cadr v))
+       ((equal tag 'INTERNAL-NUMBER) (read-back-num v))
+       ((equal tag 'INTERNAL-STRING) (read-back-string (cdr v)))
+       ((equal tag 'INTERNAL-CONS)
+	(cons (read-back (cadr v))
+	      (read-back (caddr v))))
+       (t (cons (read-back tag)
+		(read-back (cdr v)))))))))
+
+
+
+;;;;;;;;;;;;;;;;;;;;;;;;;;;;;;;;
+;;;;;;;;;;;;;;;;;;;;;;;;;;;;;;;;
+;; Global tables to keep track of
+;; all function symbols, 'boolean' function symbols,
+;; and their relational counterparts and arities
+
+(defparameter built-ins
+  '((append nil nil appendo) (reverse 1 reverso) (len 1 leno) (member 2 membero-fn)
+    (+ nil 0 do-pluso) (- 2 do-minuso) (* nil 1 do-timeso)
+    (sqr 1 do-sqro) (expt 2 do-expto)
+    (< 2 do-less-than-o-fn) (<= 2 do-less-than-equal-o-fn)
+    (> 2 do-greater-than-o-fn) (>= 2 do-greater-than-equal-o-fn)
+    (and nil t ando) (or nil nil oro) (not 1 noto)
+    (booleanp 1 booleanpo-fn) (symbolp 1 symbolpo-fn)
+    (varp 1 varpo-fn) (consp 1 conspo-fn) (symbolp 1 symbolpo-fn)
+    (endp 1 endpo-fn) (equal 2 ==-fn)
+    (listp 1 listpo-fn) (true-listp 1 true-listpo-fn)
+    (zerop 1 zeropo-fn) (numberp 1 numberpo-fn)
+    (natp 1 natpo-fn) (integerp 1 integerpo-fn) (posp 1 pospo-fn)
+    (negp 1 negpo-fn) (rationalp 1 rationalpo-fn)
+    (numerator 1 numeratoro) (denominator 1 denominatoro)
+    (stringp 1 stringpo-fn) (characterp 1 charpo-fn)
+    (string-append nil nil concato) (length 1 str-leno)
+    (subseq 3 subseqo)))
+
+
+;; if a function is known, this returns the expected arity and relation symbol,
+;; otherwise errors.
+(defun function-is-known? (fn)
+  (let ((v (assoc fn built-ins)))
+    (if v (cdr v)
+      (error "Unknown function symbol ~s" fn))))
+
+;; the same thing but for booleans
+(defparameter built-ins-bool
+  '((equal 2 ==)
+    (varp 1 varpo) (booleanp 1 booleanpo) (symbolp 1 symbolpo) (endp 1 endpo)
+    (consp 1 conspo) (stringp 1 stringpo) (characterp 1 charpo)
+    (listp 1 listpo) (true-listp 1 true-listpo)
+    (< 2 do-less-than-o) (<= 2 do-less-than-equal-o)
+    (> 2 do-greater-than-o) (>= 2 do-greater-than-equal-o)
+    (zerop 1 zeropo) (numberp 1 numberpo)
+    (natp 1 natpo) (integerp 1 integerpo) (posp 1 pospo)
+    (negp 1 negpo) (rationalp 1 rationalpo)))
+
+(defun function-is-known-bool? (fn)
+  (let ((v (assoc fn built-ins-bool)))
+    (if v (cdr v)
+      (error "Unknown boolean function symbol ~s" fn))))
